Move binding lemma to closed_meta

theories/closed_meta.v
@@ -287,4 +287,181 @@ Section Theory.
     iPureIntro; repeat split; auto.
     all: by eapply overlap_mono.
   Qed.
+
+  (** Meta theory: Generalized contexts and the binding lemma. *)
+  Definition strengthen Γ x (d: val) (D D': conn_map) := <[var x:=d]>(D ~[conn_env Γ]~> D').
+  
+  Lemma strengthen_env_generic
+        (int_ty: type → @intT_type Σ) (ϕ: conn_map → name_map → iProp Σ)
+        (Γ: env) (τ: type) x (D D': conn_map) v d (σ: gmap string val)
+        (N N': name_map)
+        (L: gset conn_name) (disj: conn_env Γ ⊥ L) (notin: var x ∉ L) O (Osub: names Γ ⊆ O)
+        (ϕ_local: Proper (overlap L ==> eq ==> (⊣⊢)) ϕ)
+        (int_local: ∀ τ, Proper (eq ==> overlap (names τ) ==> eq ==> (⊣⊢)) (int_ty τ)):
+    int_env_pre int_ty Γ D N σ -∗ (⌜N ≡[O]≡ N'⌝ ∗ int_ty τ d N' v ∗ ϕ D' N') -∗
+                let D'' := strengthen Γ x d D D' in
+                int_env_pre int_ty (<[x:=τ]>Γ) D'' N' (<[x:=v]>σ) ∗ ϕ D'' N'.
+  Proof.
+    iIntros "intΓ [eqN [intτ ϕ]]".
+    iDestruct "eqN" as %eqN; cbn.
+    iSplitR "ϕ".
+    { iDestruct "intΓ" as "[dom intΓ]".
+      iDestruct "dom" as %[domσ domD].
+      iSplit.
+      { iPureIntro; split.
+        { intros y; by rewrite !lookup_insert_is_Some domσ. }
+        { intros y.
+          rewrite /strengthen !lookup_insert_is_Some.
+          intros [<-|[neqxy iny]]; first auto.
+          right; split; first congruence.
+          rewrite lookup_merge_along_in; first auto.
+          rewrite elem_of_conn_env; exists y; auto. }
+      }
+      iIntros (x' τ' v' d' [lookupτ [lookupv lookupd]]).
+      destruct (decide (x=x')) as [<-|neq].
+      { rewrite lookup_insert in lookupd; injection lookupd as <-.
+        rewrite lookup_insert in lookupv; injection lookupv as <-.
+        rewrite lookup_insert in lookupτ; injection lookupτ as <-.
+        iFrame.
+      } {
+        rewrite lookup_insert_ne in lookupτ; last done.
+        rewrite lookup_insert_ne in lookupd; last congruence.
+        rewrite lookup_insert_ne in lookupv; last done.
+        iSpecialize ("intΓ" $! x' τ' v' d' with "[]").
+        { iPureIntro; repeat split; auto.
+          rewrite lookup_merge_along_in in lookupd; auto.
+          rewrite elem_of_conn_env.
+          exists x'; split; eauto. }
+        assert (names τ' ⊆ O).
+        { etrans; last done.
+          intros ξ inξ.
+          rewrite elem_of_names_env; eauto. }
+        iApply (int_local with "intΓ").
+        1,3: done.
+        eapply overlap_sub; done. }
+    }
+    enough (overlap L D' (<[var x:=d]>(D ~[conn_env Γ]~> D'))) as ov.
+    { by rewrite /strengthen -ov. }
+    intros n inn.
+    rewrite lookup_insert_ne.
+    2: by intros <-.
+    rewrite lookup_merge_along_not_in; first done.
+    clear -disj inn.
+    set_solver.
+  Qed.
+
+  
+  Lemma bind_existential_part (x: string) e K Γ τ₁ τ₂ η₁ η₂ η₃ A₁ A₂ (D₁ D₂ D₃: conn_map) d
+        (d_good: D₂!!RET = Some d) (Γ_names_good: names Γ ⊥ A₁)
+        (x_fresh: ∀ e', subst_ctx (<[x:=e']>∅) K = K):
+    simulation Γ e η₁ A₁ τ₁ η₂ D₁ D₂
+               -∗ simulation (<[x:=τ₁]>Γ) (fill_gctx x K) η₂ A₂ τ₂ η₃
+               (strengthen Γ x d D₁ D₂) D₃
+               -∗ simulation Γ (fill_gctx e K) η₁ (A₁ ∪ A₂) τ₂ η₃ D₁ D₃.
+  Proof.
+    iIntros "sime simK".
+    iIntros (N σ p K') "#ctx [#Γ pre] step".
+    rewrite subst_fill fill_ctx_app.
+    iMod ("sime" $! N σ p (subst_ctx (of_val <$> σ) K++K')
+          with "ctx [$Γ $pre] step") as (v₁) "[post step]".
+    iDestruct "post" as (d' N') "[props [ty pre]]".
+    iDestruct "props" as %[eqN eqd].
+    replace d' with d in * by congruence.
+    iPoseProof (strengthen_env_generic int_s_type (int_s_heap η₂) Γ τ₁ x D₁ D₂
+                                       v₁ d σ N N' (conn_heap η₂))
+      as "str".
+    { intro; rewrite elem_of_conn_env elem_of_conn_heap => [[? [? _]] [? [? _]]]; congruence. }
+    { by rewrite elem_of_conn_heap => [[? [? _]]]. }
+    { done. }
+    { intros D D' eqD ?? <-; by apply int_s_heap_local. }
+    iDestruct ("str" with "Γ [$ty $pre]") as "[Γ' pre]".
+    { iPureIntro.
+      assert (of_gset (names Γ) ⊆ not_new A₁).
+      { intro ξ.
+        rewrite elem_of_of_gset elem_of_not_new => [inξ].
+        intros []%Γ_names_good; done. }
+      apply overlap_cast, (overlap_sub (not_new A₁)); auto.
+    }
+    rewrite -fill_ctx_app -(subst_val v₁ (of_val <$> σ)) -subst_fill.
+    iMod ("simK" $! N' (<[x := v₁]>σ) p K' with "ctx [$Γ' $pre] [step]")
+      as (v₂) "[post step]".
+    { rewrite fmap_insert subst_insert_r; auto using val_closed.
+      rewrite (subst_fill (<[x:=of_val v₁]>∅)) x_fresh /= lookup_insert //. }
+    iDestruct "post" as (d'' N'') "[eqs post]".
+    iModIntro.
+    iExists v₂; iFrame.
+    iExists d'', N''; iFrame.
+    iDestruct "eqs" as %[eqN' eqd'].
+    iPureIntro; split; auto.
+    eapply overlap_trans; eauto.
+  Qed.
+
+  Lemma bind_universal_part (x: string) e e' K K' Γ τ₁ τ₂ η₁ η₂ η₃ A₁ A₂
+        (Γ_names_good: names Γ ⊥ A₁)
+        (x_fresh: ∀ e', subst_ctx (<[x:=e']>∅) K = K)
+        (x_fresh': ∀ e', subst_ctx (<[x:=e']>∅) K' = K'):
+    delayed_typed Γ η₁ e e' A₁ τ₁ η₂
+                  -∗ delayed_typed (<[x:=τ₁]>Γ) η₂ (fill_ctx x K) (fill_ctx x K') A₂ τ₂ η₃
+                  -∗ delayed_typed Γ η₁ (fill_ctx e K) (fill_ctx e' K') (A₁ ∪ A₂) τ₂ η₃.
+  Proof.
+    iIntros "dele delK".
+    iIntros (D Ni σi) "[#intΓ intη]".
+    rewrite subst_fill.
+    iApply wp_bind.
+    iSpecialize ("dele" $! D Ni σi with "[$intΓ $intη]").
+    iApply (wp_wand with "dele [-]").
+    iIntros (v) "post".
+    iDestruct "post" as (Ni' D' d') "[rel [intτ [#sim intη']]]".
+    replace (fill_ctx (of_val v) (subst_ctx (of_val <$> σi) K))
+    with (subst (of_val <$> (<[x:=v]>σi)) (fill_ctx x K)); cycle 1.
+    { rewrite fmap_insert subst_insert_r; auto using val_closed.
+      rewrite subst_fill /= lookup_insert x_fresh -(subst_val _ (of_val <$> σi)) -subst_fill.
+      rewrite subst_val //. }
+    iDestruct "rel" as %[eqN eqd].
+    iSpecialize ("delK" $! (strengthen Γ x d' D D') Ni' (<[x:=v]>σi) with "[intτ intη']").
+    { iApply (strengthen_env_generic
+                int_i_type (int_i_heap η₂) Γ τ₁ x D D' v d' σi Ni Ni' (conn_heap η₂)
+              with "intΓ [intτ intη']").
+      - intro n.
+        rewrite elem_of_conn_env elem_of_conn_heap => [[? [? _]] [? [? _]]]; congruence.
+      - rewrite elem_of_conn_heap => [[? [? _]]]; done.
+      - done.
+      - intros D₁ D₂ eqD ?? <-.
+        apply int_i_heap_local; auto; done.
+      - iFrame.
+        iPureIntro.
+        assert (of_gset (names Γ) ⊆ not_new A₁).
+        { intro ξ; rewrite elem_of_of_gset elem_of_not_new; exact (Γ_names_good ξ). }
+        apply overlap_cast, (overlap_sub (not_new A₁)); auto.
+    }
+    iApply (wp_wand with "delK").
+    iIntros (v') "post".
+    iDestruct "post" as (Ni'' D'' d'') "[pure [intτ [#sim' intη]]]".
+    iDestruct "pure" as %[eqN' eqD'].
+    iExists Ni'', D'', d''; iFrame.
+    iSplit.
+    { iPureIntro; repeat split; eauto using overlap_trans. }
+    iAlways.
+    iApply (bind_existential_part with "sim sim'"); auto.
+  Qed.
+
+  Lemma delayed_bind
+        (x: string) e e' K K' Γ τ₁ τ₂ η₁ η₂ η₃ U A₁ A₂
+        (x_fresh: ∀ e', subst_ctx (<[x:=e']>∅) K = K)
+        (x_fresh': ∀ e', subst_ctx (<[x:=e']>∅) K' = K')
+        (dele: delayed_simulation U Γ η₁ e e' A₁ τ₁ η₂)
+        (delK: delayed_simulation (U ∪ A₁) (<[x:=τ₁]>Γ) η₂ (fill_ctx x K) (fill_ctx x K') A₂ τ₂ η₃):
+    delayed_typed Γ η₁ (fill_ctx e K) (fill_ctx e' K') (A₁ ∪ A₂) τ₂ η₃.
+  Proof.
+    destruct dele as [namese tye tye' dele].
+    destruct delK as [namesK tyK tyK' delK].
+    iApply bind_universal_part.
+    2,3: done.
+    2: iApply dele.
+    2: iApply delK.
+    apply typing_good_names in tye.
+    2,3: clear -namese; set_solver.
+    set_solver.
+  Qed.
+
 End Theory.
